engine/PrisonersDilemma.lean
@@ -206,4 +206,6 @@ import PrisonersDilemma.Tau.Theorems.TauEBot.Phase
 import PrisonersDilemma.Tau.Theorems.TauJust.Phase
 import PrisonersDilemma.Tau.Theorems.TauOBot.Phase
 import PrisonersDilemma.Tau.Theorems.TauGuardian.Phase
+import PrisonersDilemma.Tau.Theorems.TauDBot.Helpers
+import PrisonersDilemma.Tau.Theorems.TauDBot.Phase
 import PrisonersDilemma.Tau.Theorems.Matrix
